one line solve_decoder for 8.4pl6

src/BinEncoders/Env/BinLib/Char.v
@@ -21,7 +21,7 @@ Section CharBinEncoder.
   Defined.
 
   Definition Char_encode (c : ascii) (ce : CacheEncode) :=
-    FixInt_encode cacheAdd (FixInt_of_ascii c) ce.
+    FixInt_encode (FixInt_of_ascii c) ce.
 
   Definition Char_decode (b : list bool) (cd : CacheDecode) :=
     let (x, e) := FixInt_decode 8 cacheAdd b cd in
@@ -52,3 +52,5 @@ Global Instance Char_decoder cache cacheAdd predicate
   : decoder cache btransformer predicate (@Char_encode cache cacheAdd) :=
   { decode := @Char_decode cache cacheAdd;
     decode_correct := @Char_encode_correct _ _ _ }.
+
+Arguments Char_encode {_ _} _ _.
